theories/fundamental.v
@@ -32,7 +32,7 @@ Section fundamental.
     iIntros "[[Hfull Hreg] [Hmreg [Hr [Hsts Hown]]]]".
 
     assert ( readAllowed p = true \/ readAllowed p = false )
-      as [Hread_p|Hread_p] by (destruct p ; naive_solver)
+      as [Hread_p|Hread_p] by (destruct_perm p ; naive_solver)
     ; cycle 1.
     { (* if p not readable, then execution will fail *)
       iDestruct "Hfull" as "%". iDestruct "Hreg" as "#Hreg".
@@ -88,10 +88,13 @@ Section fundamental.
     iPoseProof "Hinv_interp" as "#Hinv".
     iEval (rewrite !fixpoint_interp1_eq interp1_eq) in "Hinv".
     rewrite decide_False; last (destruct p ; naive_solver).
-    rewrite decide_False; last (destruct p ; naive_solver).
+    destruct (isSentry p) eqn:Hsentryp; first (destruct_perm p ; naive_solver).
     iDestruct "Hinv" as "[#Hinv %Hpwl_cond]".
 
     iDestruct (extract_from_region_inv _ _ a with "Hinv") as "H";auto.
+    rewrite ExecPCPerm_readAllowed; auto.
+    2: { rewrite /ExecPCPerm; destruct_perm p ; naive_solver. }
+
     iDestruct (write_allowed_implies_ra with "[Hreg] [H]")
       as (p'' P'' Hflp'' Hperscond_P'') "(Hrela & Hzcond & Hrcond & Hwcond & %Hstate_a)"
     ;auto; iClear "Hinv H".
